---
title: "First 2 week update~~"
author: "benjamin chu"
date: "5/12/2018"
---

```{r setup, include=FALSE}
knitr::opts_chunk$set(echo = TRUE)
```

Hi everyone, two weeks no see.

The past 2 weeks have been the community bonding period of google summer of codes. I have made several updates in the JSOC-standup channel on slack, asked some questions on julia discourse, and wrote some code for my Ph.D advisor. My coding was not directly related to my project, but it helped me understand the codebase of [MendelBase](https://openmendel.github.io/MendelBase.jl/) and [SnpArrays](https://openmendel.github.io/SnpArrays.jl/latest/) much better, so yayyyyy.

Other than that, I probably spent a disproportionate amount of time on my current course [convex optimization](http://www.seas.ucla.edu/~vandenbe/ee236b/ee236b.html). In this respect, I thought I'd share one of the problems I did on my previous homework (hw5, which is 3.11.d in the textbook).

**Problem:**

Let $x \in \mathbb{R}^n$ and $F(x) = F_0 + x_1F_1 + ... + x_nF_n$ with $F_i$ being symmertic $m \times m$ matrices. The domain of $f$ in each subproblem is $dom f = \{x \in \mathbb{R}^n \ | \ F(x) \text{ is positive definite}\}$. Formulate the following minimization problem as a *semi-definite program* (that is, a minimization problem with linear objective function and linear matrix inequalities):

\begin{align*}
		&\text{minimize} \ \quad f(x) = E(c^TF(x)^{-1}c)
\end{align*}

where $c$ is a random vector with mean $E(c) = \bar{c}$ and covariance $E(c - \bar{c})(c - \bar{c})^T = S.$

**Solution**

Note that covariance matrices are always symmetric, so $S = Q\Lambda Q^T = \sum \lambda_i q_iq_i^T$. Using cyclic permutation of the trace operator, we have
\begin{align*}
	E(c^TF(x)^{-1}c) &= E(tr(c^TF(x)^{-1}c)) = E(tr(F(x)^{-1}cc^T)) = tr(F(x)^{-1}E(cc^T))\\
	&= tr(F(x)^{-1}S) = tr(F(x)^{-1}(\sum_{i=1}^n \lambda_iq_iq_i^T)) = tr(\sum_{i=1}^n \lambda_i F(x)^{-1} q_iq_i^T)\\
	&= \sum_{i=1}^n \lambda_iq_i^T F(x)^{-1} q_i
\end{align*}
Thus we have 
\begin{align*}
	& \begin{cases}
		&\text{minimize} \ \quad   E(c^TF(x)^{-1}c)\\
	\end{cases}
	\iff \begin{cases}
		\text{minimize} \ \quad \sum_{i=1}^n \lambda_iq_i^T F(x)^{-1} q_i  \\
	\end{cases}\\
	\iff &\begin{cases}
		&\text{minimize} \ \quad   \sum_{i=1}^n \lambda_i t\\
		&\text{subject to} \quad t \geq q_i^TF(x)^{-1}q_i
	\end{cases}
	\iff \begin{cases}
		&\text{minimize} \ \quad   \sum_{i=1}^n \lambda_i t\\
		&\text{subject to} \quad \begin{bmatrix}
			F(x) & q_i \\ q_i^T & t
		\end{bmatrix} \text{ is positive definite}
	\end{cases}\\
		\iff &\begin{cases}
		&\text{minimize} \ \quad   \sum_{i=1}^n \lambda_i t\\
		&\text{subject to} \quad 
		\begin{bmatrix}
			F_0 & 0\\
			0 & 0
		\end{bmatrix}	 + ... + x_n \begin{bmatrix}
			F_n & 0\\0 & 0
		\end{bmatrix} + t \begin{bmatrix}
			0 & 0 \\ 0 & 1
		\end{bmatrix} + \begin{bmatrix}
			0 & q_i\\ q_i^T & 0
		\end{bmatrix}
	\end{cases} 
\end{align*}
which is of the linear matrix inequality form we desire. Note the second to last if-and-only-if is by the property of Schur complement. This completes the proof. 